thys/Untyped_Lambda_Calculus/ILC.thy
@@ -865,38 +865,38 @@ by (auto simp: iterm_pre.supp_comp_bound)
 
 (* "making" the substitution function that maps each xs_i to es_i; only 
 meaningful if xs is non-repetitive *)
-definition "mkSubst xs es \<equiv> \<lambda>x. if x \<in> dsset xs then snth es (dtheN xs x) else iVar x"
+definition "imkSubst xs es \<equiv> \<lambda>x. if x \<in> dsset xs then snth es (dtheN xs x) else iVar x"
 
-lemma mkSubst_dsnth[simp]: "mkSubst xs es (dsnth xs i) = snth es i"
-unfolding mkSubst_def using dsset_range by auto
+lemma imkSubst_dsnth[simp]: "imkSubst xs es (dsnth xs i) = snth es i"
+unfolding imkSubst_def using dsset_range by auto
 
-lemma mkSubst_idle[simp]: "\<not> x \<in> dsset xs \<Longrightarrow> mkSubst xs es x = iVar x"
-unfolding mkSubst_def by auto
+lemma imkSubst_idle[simp]: "\<not> x \<in> dsset xs \<Longrightarrow> imkSubst xs es x = iVar x"
+unfolding imkSubst_def by auto
 
 lemma card_dsset_ivar: "|dsset xs| <o |UNIV::ivar set|"
 using countable_card_ivar countable_card_le_natLeq dsset_natLeq by auto
 
-lemma SSupp_mkSubst[simp,intro]: "|SSupp (mkSubst xs es)| <o |UNIV::ivar set|"
+lemma SSupp_imkSubst[simp,intro]: "|SSupp (imkSubst xs es)| <o |UNIV::ivar set|"
 proof-
-  have "SSupp (mkSubst xs es) \<subseteq> dsset xs"
-  unfolding SSupp_def by auto (metis mkSubst_idle)
+  have "SSupp (imkSubst xs es) \<subseteq> dsset xs"
+  unfolding SSupp_def by auto (metis imkSubst_idle)
   thus ?thesis by (simp add: card_of_subset_bound card_dsset_ivar)
 qed
 
-lemma mkSubst_smap_rrename: 
+lemma imkSubst_smap_rrename: 
 assumes s: "bij (\<sigma>::ivar\<Rightarrow>ivar)" "|supp \<sigma>| <o |UNIV::ivar set|" 
-shows "mkSubst (dsmap \<sigma> xs) (smap (rrename \<sigma>) es2) \<circ> \<sigma> = rrename \<sigma> \<circ> mkSubst xs es2"
+shows "imkSubst (dsmap \<sigma> xs) (smap (rrename \<sigma>) es2) \<circ> \<sigma> = rrename \<sigma> \<circ> imkSubst xs es2"
 proof(rule ext)  
   fix x
   have inj[simp]: "inj_on \<sigma> (dsset xs)"
   using s unfolding bij_def inj_on_def by auto
-  show "(mkSubst (dsmap \<sigma> xs) (smap (rrename \<sigma>) es2) \<circ> \<sigma>) x = (rrename \<sigma> \<circ> mkSubst xs es2) x"
+  show "(imkSubst (dsmap \<sigma> xs) (smap (rrename \<sigma>) es2) \<circ> \<sigma>) x = (rrename \<sigma> \<circ> imkSubst xs es2) x"
   proof(cases "x \<in> dsset xs")
     case False
     hence F: "\<not> \<sigma> x \<in> dsset (dsmap \<sigma> xs)"
     using s by auto
     thus ?thesis using F False
-    unfolding o_def apply(subst mkSubst_idle) 
+    unfolding o_def apply(subst imkSubst_idle) 
       subgoal by auto
       subgoal using s by auto .
   next
@@ -905,28 +905,28 @@ proof(rule ext)
     hence Ti: "\<sigma> x = dsnth (dsmap \<sigma> xs) i"
     using s dsmap_alt inj by blast
     thus ?thesis 
-    unfolding o_def Ti apply(subst mkSubst_dsnth) 
+    unfolding o_def Ti apply(subst imkSubst_dsnth) 
     unfolding Tri by auto 
   qed
 qed
 
-lemma mkSubst_smap_rrename_inv: 
+lemma imkSubst_smap_rrename_inv: 
 assumes "bij (\<sigma>::ivar\<Rightarrow>ivar)" "|supp \<sigma>| <o |UNIV::ivar set|" 
-shows "mkSubst (dsmap \<sigma> xs) (smap (rrename \<sigma>) es2) = rrename \<sigma> \<circ> mkSubst xs es2 o inv \<sigma>"
-unfolding mkSubst_smap_rrename[OF assms, symmetric] using assms unfolding fun_eq_iff by auto
+shows "imkSubst (dsmap \<sigma> xs) (smap (rrename \<sigma>) es2) = rrename \<sigma> \<circ> imkSubst xs es2 o inv \<sigma>"
+unfolding imkSubst_smap_rrename[OF assms, symmetric] using assms unfolding fun_eq_iff by auto
 
-lemma card_SSupp_itvsubst_mkSubst_rrename_inv: 
+lemma card_SSupp_itvsubst_imkSubst_rrename_inv: 
 "bij (\<sigma>::ivar\<Rightarrow>ivar) \<Longrightarrow> |supp \<sigma>| <o |UNIV::ivar set| \<Longrightarrow> 
- |SSupp (itvsubst (rrename \<sigma> \<circ> mkSubst xs es \<circ> inv \<sigma>) \<circ> (iVar \<circ> \<sigma>))| <o |UNIV::ivar set|"
-by (metis SSupp_itvsubst_bound SSupp_mkSubst mkSubst_smap_rrename_inv supp_SSupp_iVar_le)
+ |SSupp (itvsubst (rrename \<sigma> \<circ> imkSubst xs es \<circ> inv \<sigma>) \<circ> (iVar \<circ> \<sigma>))| <o |UNIV::ivar set|"
+by (metis SSupp_itvsubst_bound SSupp_imkSubst imkSubst_smap_rrename_inv supp_SSupp_iVar_le)
 
-lemma card_SSupp_mkSubst_rrename_inv: 
+lemma card_SSupp_imkSubst_rrename_inv: 
 "bij (\<sigma>::ivar\<Rightarrow>ivar) \<Longrightarrow> |supp \<sigma>| <o |UNIV::ivar set|  \<Longrightarrow> 
-|SSupp (rrename \<sigma> \<circ> mkSubst xs es2 \<circ> inv \<sigma>)| <o |UNIV::ivar set|"
-by (metis SSupp_mkSubst mkSubst_smap_rrename_inv)
+|SSupp (rrename \<sigma> \<circ> imkSubst xs es2 \<circ> inv \<sigma>)| <o |UNIV::ivar set|"
+by (metis SSupp_imkSubst imkSubst_smap_rrename_inv)
 
-lemma mkSubst_smap: "bij f \<Longrightarrow> z \<in> dsset xs \<Longrightarrow> mkSubst (dsmap f xs) es (f z) = mkSubst xs es z"
-by (metis bij_betw_def bij_imp_bij_betw dsmap_alt dtheN mkSubst_dsnth) 
+lemma imkSubst_smap: "bij f \<Longrightarrow> z \<in> dsset xs \<Longrightarrow> imkSubst (dsmap f xs) es (f z) = imkSubst xs es z"
+by (metis bij_betw_def bij_imp_bij_betw dsmap_alt dtheN imkSubst_dsnth) 
 
 
 end
