thys/Untyped_Lambda_Calculus/ILC2.thy
@@ -1,0 +1,21 @@
+theory ILC2 
+imports ILC "../Generic_Barendregt_Enhanced_Rule_Induction"
+begin
+
+(* INSTANTIATING THE Small LOCALE (INDEPENDENTLY OF THE CONSIDERED INDUCTIVE PREDICATE *) 
+
+print_locales
+interpretation Small where dummy = "undefined :: ivar" 
+apply standard
+  apply (simp add: infinite_ivar)
+  using regularCard_ivar .  
+
+lemma small_dsset[simp,intro]: "small (dsset xs)"
+by (simp add: card_dsset_ivar small_def)
+
+lemma small_image_sset[simp,intro]: "inj_on f (dsset xs) \<Longrightarrow> small (f ` dsset xs)"
+by (metis countable_card_ivar countable_card_le_natLeq dsset.rep_eq small_def sset_natLeq stream.set_map)
+
+
+
+end 
