thys/Untyped_Lambda_Calculus/LC2.thy
@@ -1,0 +1,13 @@
+theory LC2 
+imports LC "../Generic_Barendregt_Enhanced_Rule_Induction"
+begin
+
+(* INSTATIATING THE Small LOCALE (INDEPENDENTLY OF THE CONSIDERED INDUCTIVE PREDICATE *) 
+
+print_locales
+interpretation Small where dummy = "undefined :: var" 
+apply standard
+  apply (simp add: infinite_var)  
+  using var_term_pre_class.regular by blast
+
+end
